src/dafny/util/stack.dfy
@@ -27,44 +27,44 @@ module Stack {
     witness Stack([])
 
     // Get number of items currently on this Stack.
-    function method size(st:T) : nat { |st.contents| }
+    function method Size(st:T) : nat { |st.contents| }
 
     // Get remaining capacity of stack (i.e. number of items we could
     // still push).
-    function method capacity(st:T) : nat {
+    function method Capacity(st:T) : nat {
       CAPACITY - |st.contents|
     }
 
     // Create an empty stack.
-    function method create() : T { Stack(contents:=[]) }
+    function method Create() : T { Stack(contents:=[]) }
 
     // Push word onto Stack.  This requires that there is sufficient
     // space for that item.
-    function method push(st:T, val:u256) : T
+    function method Push(st:T, val:u256) : T
         // Sanity check enough space.
-        requires size(st) < CAPACITY {
+        requires Size(st) < CAPACITY {
             Stack(contents:=([val] + st.contents))
     }
 
     // Peek nth word from top of Stack (where 0 is top item, 1 is next
     // item, and so on).  This requires there are sufficiently many
     // words.
-    function method peek(st:T, k:int) : u256
+    function method Peek(st:T, k:int) : u256
         // Sanity check enough items to pop!
-        requires k >= 0 && k < size(st) {
+        requires k >= 0 && k < Size(st) {
             st.contents[k]
     }
 
     // Pop word off of this Stack.  This requires something to pop!
-    function method pop(st:T) : T
+    function method Pop(st:T) : T
         // Sanity check something to pop.
-        requires size(st) > 0 {
+        requires Size(st) > 0 {
             Stack(contents:=st.contents[1..])
     }
 
     // Swap top item and kth item
-    function method swap(st:T, k:nat) : T
-      requires size(st) > k {
+    function method Swap(st:T, k:nat) : T
+      requires Size(st) > k {
         var top := st.contents[0];
         var kth := st.contents[k];
         Stack(contents:=st.contents[0:=kth][k:=top])
